src/twolang/simp.v
@@ -1,6 +1,6 @@
 (** this file just gather up all the imports needed to work with simp_lang *)
 From iris.proofmode Require Export tactics.
-From iris_simp_lang Require Export
+From twolang Require Export
      notation class_instances primitive_laws proofmode.
 From iris Require Import options.
 Export lang.
